lambda.v
@@ -1,0 +1,265 @@
+Require Import Arith.
+Require Import Omega.
+Require Import Recdef.
+Require Import ZArith.
+Require FMapList.
+Require Import OrderedType OrderedTypeEx.
+Require Import Strings.String.
+Require Import Strings.Ascii.
+Require Import Coq.Program.Tactics.
+Import ListNotations.
+
+Load parse.
+
+(* Lambda Calculus with 0-indexed De Bruijn indices *)
+Inductive Lambda : Set :=
+| l_var : nat -> Lambda
+| l_lam : Lambda -> Lambda
+| l_app : Lambda -> Lambda -> Lambda.
+
+Function lambda_replace (e: Lambda) (x: Lambda) (n: nat): Lambda :=
+  match e with
+  | l_var m => if m =? n then x else e
+  | l_lam e' => l_lam (lambda_replace e' x (S n))
+  | l_app e1 e2 => l_app (lambda_replace e1 x n) (lambda_replace e2 x n)
+  end.
+
+(* TODO: Do we want CBV instead? *)
+Function lambda_step (e: Lambda): option Lambda :=
+  match e with
+  | l_var _ => None
+  | l_lam e' =>
+    match lambda_step e' with
+    | Some e'' => Some (l_lam e'')
+    | None => None
+    end
+  | l_app (l_lam e1) e2 => Some (lambda_replace e1 e2 0)
+  | l_app e1 e2 =>
+    match lambda_step e1 with
+    | Some e1' => Some (l_app e1' e2)
+    | None =>
+      match lambda_step e2 with
+      | Some e2' => Some (l_app e1 e2')
+      | None => None
+      end
+    end
+  end.
+
+Function lambda_run (e: Lambda) (fuel: nat): option Lambda :=
+  match fuel with
+  | 0 => None
+  | S f =>
+    match lambda_step e with
+    | None => Some e
+    | Some e' => lambda_run e' f
+    end
+  end.
+
+Section LambdaParsing.
+
+  Local Inductive LambdaTree : Set :=
+  | lam_end
+  | lam_lam (t: LambdaTree)
+  | lam_dot (t: LambdaTree)
+  | lam_wsp (t: LambdaTree)
+  | lam_id (str: string) (t: LambdaTree)
+  | lam_paren (inner: LambdaTree) (t: LambdaTree).
+
+  Local Definition ParseState := @Parse.ParseState LambdaTree.
+
+  Function parse_lambdatree_state (l: list ascii): ParseState :=
+    match l with
+    | [] => Parse.ok lam_end []
+    | hd :: tl =>
+      match parse_lambdatree_state tl with
+      | Parse.error => Parse.error
+      | Parse.ok cur stack =>
+        match hd with
+        | "032"%char
+        | "009"%char
+        | "010"%char
+        | "013"%char =>
+          match cur with
+          | lam_wsp _ => Parse.ok cur stack
+          | _ => Parse.ok (lam_wsp cur) stack
+          end
+        | "\"%char => Parse.ok (lam_lam cur) stack
+        | "."%char => Parse.ok (lam_dot cur) stack
+        | ")"%char => Parse.ok (lam_end) (cur :: stack)
+        | "("%char =>
+          match stack with
+          | [] => Parse.error
+          | next :: stack' => Parse.ok (lam_paren cur next) stack'
+          end
+        | _ =>
+          match cur with
+          | lam_id str next => Parse.ok (lam_id (String hd str) next) stack
+          | _ => Parse.ok (lam_id (String hd EmptyString) cur) stack
+          end
+        end
+      end
+    end.
+
+  Function lambda_strip_wsp (t: LambdaTree): LambdaTree :=
+    match t with
+    | lam_end => lam_end
+    | lam_wsp t' => lambda_strip_wsp t'
+    | lam_lam t' => lam_lam (lambda_strip_wsp t')
+    | lam_dot t' => lam_dot (lambda_strip_wsp t')
+    | lam_id s t' => lam_id s (lambda_strip_wsp t')
+    | lam_paren inner t' =>
+      lam_paren (lambda_strip_wsp inner) (lambda_strip_wsp t')
+    end.
+
+  Local Inductive NamedLambda : Set :=
+  | nl_var (s: string)
+  | nl_lam (s: string) (e: NamedLambda)
+  | nl_app (e1: NamedLambda) (e2: NamedLambda).
+
+  Function app_of_lambda_list (ls: list NamedLambda) {measure List.length ls}:
+    option NamedLambda :=
+    match ls with
+    | [] => None
+    | e :: [] => Some e
+    | e1 :: e2 :: tl => app_of_lambda_list ((nl_app e1 e2) :: tl)
+    end.
+  intuition.
+  Defined.
+
+  Function named_lambda_of_tree (acc: list NamedLambda) (t: LambdaTree):
+    option NamedLambda :=
+    match t with
+    | lam_end => app_of_lambda_list (rev acc)
+    | lam_wsp _ => None
+    | lam_lam (lam_id s (lam_dot t')) =>
+      match  named_lambda_of_tree [] t' with
+      | None => None
+      | Some e => Some (nl_lam s e)
+      end
+    | lam_lam _ | lam_dot _ => None
+    | lam_id s t' => named_lambda_of_tree (nl_var s :: acc) t'
+    | lam_paren inner t' =>
+      match named_lambda_of_tree [] inner with
+      | None => None
+      | Some e => named_lambda_of_tree (e :: acc) t'
+      end
+    end.
+
+  Function parse_named_lambda (s: string): option NamedLambda :=
+    match parse_lambdatree_state (Parse.chars_of_string s) with
+    | Parse.error => None
+    | Parse.ok cur stack =>
+      match stack with
+      | _ :: _ => None
+      | [] => named_lambda_of_tree [] (lambda_strip_wsp cur)
+      end
+    end.
+
+  Example named_id: parse_named_lambda "\x.x" = Some (nl_lam "x" (nl_var "x")).
+  auto. Qed.
+
+  Example named_true:
+    parse_named_lambda "\x.\y.x" = Some (nl_lam "x" (nl_lam "y" (nl_var "x"))).
+  auto. Qed.
+
+  Example named_false:
+    parse_named_lambda " \ x . \ y  .  (y  ) " =
+    Some (nl_lam "x" (nl_lam "y" (nl_var "y"))).
+  auto. Qed.
+
+  Example named_Y:
+    parse_named_lambda "\f.(\x.f (x x)) (\x.f (x x))" =
+    let fn_app := nl_app (nl_var "f") (nl_app (nl_var "x") (nl_var "x")) in
+    Some (nl_lam "f" (nl_app (nl_lam "x" fn_app) (nl_lam "x" fn_app))).
+  auto. Qed.
+
+  Example named_parens:
+    parse_named_lambda "(((\x.(((x))))))" = Some (nl_lam "x" (nl_var "x")).
+  auto. Qed.
+
+  Example named_apps:
+    parse_named_lambda "x y z w" =
+    Some (nl_app (
+              nl_app (
+                  nl_app (nl_var "x") (nl_var "y")
+                ) (nl_var "z")
+            ) (nl_var "w")).
+  auto. Qed.
+
+  Example named_bad_lambdas: parse_named_lambda "\\x.x" = None.
+  auto. Qed.
+
+  Example named_bad_dots: parse_named_lambda "\x..x" = None.
+  auto. Qed.
+
+  Example named_bad_parens: parse_named_lambda "\x.((x)" = None.
+  auto. Qed.
+
+  Example named_bad_parens2: parse_named_lambda "\x.x ()" = None.
+  auto. Qed.
+
+  Function index_of (x: string) (l: list string): option nat :=
+    match l with
+    | [] => None
+    | hd :: tl =>
+      if string_dec hd x then Some 0
+      else match index_of x tl with
+           | Some i => Some (S i)
+           | None => None
+           end
+    end.
+
+  Function lambda_strip_names (l: NamedLambda) (xs: list string):
+    option Lambda :=
+    match l with
+    | nl_var x =>
+      match index_of x xs with
+      | Some n => Some (l_var n)
+      | None => None
+      end
+    | nl_lam x e =>
+      let stripped := lambda_strip_names e (x :: xs) in
+      match stripped with
+      | Some e' => Some (l_lam e')
+      | None => None
+      end
+    | nl_app e1 e2 =>
+      let stripped := (lambda_strip_names e1 xs, lambda_strip_names e2 xs) in
+      match stripped with
+      | (Some e1', Some e2') => Some (l_app e1' e2')
+      | _ => None
+      end
+    end.
+
+  Function parse_lambda (s: string): option Lambda :=
+    match parse_named_lambda s with
+    | None => None
+    | Some nl => lambda_strip_names nl []
+    end.
+
+  Example lambda_id: parse_lambda "\x.x" = Some (l_lam (l_var 0)).
+  auto. Qed.
+
+  Example lambda_true:
+    parse_lambda "\x.\y.x" = Some (l_lam (l_lam (l_var 1))).
+  auto. Qed.
+
+  Example lambda_false:
+    parse_lambda " \ x . \ y  .  (y  ) " =  Some (l_lam (l_lam (l_var 0))).
+  auto. Qed.
+
+  Example lambda_Y:
+    parse_lambda "\f.(\x.f (x x)) (\x.f (x x))" =
+    let fn_app := l_app (l_var 1) (l_app (l_var 0) (l_var 0)) in
+    Some (l_lam (l_app (l_lam fn_app) (l_lam fn_app))).
+  auto. Qed.
+
+  Example lambda_parens:
+    parse_lambda "(((\x.(((x))))))" = Some (l_lam (l_var 0)).
+  auto. Qed.
+
+  Example lambda_apps:
+    parse_lambda "x y z w" = None.
+  auto. Qed.
+
+End LambdaParsing.
