parse.v
@@ -1,0 +1,32 @@
+Require Import Strings.String.
+Require Import Strings.Ascii.
+Require Import OrderedType OrderedTypeEx.
+Import ListNotations.
+
+Module Parse.
+
+  Inductive ParseState {AST: Type}: Type :=
+  | ok (cur: AST) (stack: list AST)
+  | error.
+
+  Function chars_of_string (str: string): list ascii :=
+    match str with
+    | EmptyString => []
+    | String a str' => a :: (chars_of_string str')
+    end.
+
+  Function string_of_chars (l: list ascii): string :=
+    match l with
+    | [] => EmptyString
+    | a :: l' => String a (string_of_chars l')
+    end.
+
+  Lemma chars_of_string_of_chars_inv (l: list ascii):
+    chars_of_string (string_of_chars l) = l.
+  Proof.
+    induction l; auto.
+    rewrite string_of_chars_equation, chars_of_string_equation.
+    now rewrite IHl.
+  Qed.
+
+End Parse.
